systems/ChordProof.v
@@ -25,6 +25,36 @@ Close Scope boolean_if_scope.
 Open Scope general_if_scope.
 Open Scope string_scope.
 
+Definition has_pred (gst : global_state) (h : addr) (p : option pointer) : Prop :=
+  exists st,
+    sigma gst h = Some st /\
+    pred st = p.
+
+Lemma has_pred_intro :
+  forall gst h p st,
+    sigma gst h = Some st ->
+    pred st = p ->
+    has_pred gst h p.
+Proof.
+  unfold has_pred.
+  eauto.
+Qed.
+
+Definition has_first_succ (gst : global_state) (h : addr) (s : pointer) : Prop :=
+  exists st,
+    sigma gst h = Some st /\
+    hd_error (succ_list st) = Some s.
+
+Lemma has_first_succ_intro :
+  forall gst h s st,
+    sigma gst h = Some st ->
+    hd_error (succ_list st) = Some s ->
+    has_first_succ gst h s.
+Proof.
+  intros.
+  eexists; eauto.
+Qed.
+
 Definition timeouts_detect_failure (gst : global_state) : Prop :=
   forall xs t ys h dead req,
     (trace gst) = xs ++ t :: ys ->
